\begin{document}
V\cdot \frac{dc(t)}{dt} = q\cdot A_{1} - u\cdot A_{2}\cdot c(t)
\newline
\newline
	given\hspace{0.5cm} q\cdot A_{1} = E\hspace{0.5cm}
\newline mark\hspace{0.5cm} \alpha = u\cdot A_{2}
\newline
c(t) = const\cdot e^{\frac{-\alpha \cdot t}{V}}+\frac{E}{\alpha}
\newline
\int \frac{V\cdot{dc(t)}}{E-\alpha\cdot c(t)}dc = \int dt
\newline
\frac{-V}{\alpha}\cdot\ln (E-\alpha\cdot c(t)) +C_1 = t + C_2 
\newline
\newline
c(t) = C^*\cdot\exp (\frac{\alpha\cdot t}{V})+\frac{E}{\alpha} 
\end{document}

V\cdot \frac{dc(t)}{dt} = E - \alpha \cdot c(t)
\newline
\newline
E(t) = \left\{\begin{matrix}
	\hspace{0.0000001cm}684\cdot10^{9}\hspace{0.2cm}\frac{\mu g}{h}  \hspace{1cm} t=\left \{ 1-3,11-13 \right \}& \\ 
	\hspace{1cm}0  \hspace{2.9cm} t=\left \{ 0,4-10,14-23 \right \}& 
\end{matrix}\right.
\newline
c(t) = C_1\cdot exp(\frac{-\alpha \cdot t}{V})


c(t) = -21.11*\cdot\exp (-1.029\cdot t)+\frac{E}{\alpha} 

c(t) = -126.67*\cdot\exp (-1.029\cdot t)+126.67

c(t) = 110.5\cdot\exp (-1.029\cdot t)


cc = c^*\cdot exp(-1.029\tau)-c^*
\newline
\newline
\frac{1}{\frac{cc}{c^*}+1} = exp(1.029\tau)
\newline
\newline
\tau = \frac{1}{1.029}[ln(\frac{c^*}{cc+c^*})]

V\cdot \frac{dc(t)}{dt} = E - \alpha\cdot c(t) - r\cdot V\cdot c(t)
\newline
\newline
\newline mark\hspace{0.5cm} \beta= \alpha+r \cdot V
\newline
\newline
\int \frac{V\cdot{dc(t)}}{E-\beta\cdot c(t)}dc = \int dt
\newline
\newline
\frac{-V}{\beta}\cdot\ln (E-\beta\cdot c(t)) +C_1 = t + C_2 
\newline
\newline
c(t) = C^*\cdot\exp (-\frac{\beta\cdot t}{V})+\frac{E}{\beta} 

c(t) = -3.6\cdot10^{-6} \cdot\exp (6 \cdot 10^{6}\cdot t)+3.6\cdot10^{-6} 
